checker/mTypes.mli
@@ -8,10 +8,14 @@ type vprop =
 | ILe of ivar*int
 | IEq of ivar*int
 | BTrue of bvar
+| CTrue (* Constant true. *)
 
 type lit =
 | Pos of vprop
 | Neg of vprop
+
+type bound = (ivar * int) * int
+type bounds = bound list
 
 val negate : lit -> lit
 
