checker/model.mli
@@ -23,3 +23,5 @@ val get_checker : t -> MTypes.ident -> Checker.t
 val string_of_vprop : t -> MTypes.vprop -> string
 val string_of_lit : t -> MTypes.lit -> string
 val string_of_clause : t -> MTypes.clause -> string
+
+val get_bounds : t -> MTypes.bounds
