checker/checker_impl.v
@@ -12,7 +12,11 @@ Set Extraction Optimize.
 Extraction "checker_impl.ml"
   prim.check_inf prim.check_clause
   cumulative.check_cumul
+  cumulative.check_cumul_tt
+  cumulative.check_cumul_bnd
   reif.check_reif
   linear.check_lincon
+  linear.check_linear_bnd
   element.check_element
+  element.check_element_bnd
   nat_of_int int_of_nat.
